\section*{Exercise 1.3}

Consider a Lyapunov function \( V(x)=x_{1}^{2}+x_{2}^{2} \) for the following DS
\begin{equation*}
    \dot{x}_{1}=-x_{1}+x_{1} x_{2}, \quad \dot{x}_{2}=-x_{2}
\end{equation*}
\begin{enumerate}[noitemsep]
    \item Find the equilibrium point
    \item Find a region of attraction and show that the equilibrium point is asymptotically stable
\end{enumerate}

\subsection*{Solution}

\subsection*{1. Equilibrium point}

The given system is a nonlinear system whose equilibrium point can be found by,
\[
    \implies
    \dot{x}_{2} = -x_{2} = 0
    \implies
    x_{2} = 0
\]
\[
    \implies
    \dot{x}_{1} = -x_{1} + x_{1} x_{2} = 0
    \implies
    x_{1} = 0 \text{ or } x_{2} = 1 (\text{rejected})
\]
Therefore, the \underline{equilibrium point} is at \( \boxed{ (0, 0) } \).

\subsection*{2. Region of attraction and stability}

Given the Lyapunov function \( V(x) = x_{1}^{2} + x_{2}^{2} \), we can see that it is positive definite, i.e., \( V(x) > 0 \) for all \( x \neq 0 \) and \( V(0) = 0 \).
The derivative of \( V(x) \) can be found as,
\[
    \dot{V}(x) = \nabla V(x) \cdot f(x)
    \quad \text{where} \quad
    f(x) = \begin{bmatrix} -x_{1} + x_{1} x_{2} \\ -x_{2} \end{bmatrix}
\]
\[
    \implies
    \dot{V}(x) = \begin{bmatrix} 2x_{1} & 2x_{2} \end{bmatrix}
    \begin{bmatrix} -x_{1} + x_{1} x_{2} \\ -x_{2} \end{bmatrix}
    = -2x_{1}^{2} + 2x_{1}^{2} x_{2} - 2x_{2}^{2}
    = -2(x_{1}^{2} + x_{2}^{2}) + 2x_{1}^{2} x_{2}
\]
The first term here \( -2(x_{1}^{2} + x_{2}^{2}) \) is always negative definite, but due to the presence of the term \( 2x_{1}^{2} x_{2} \), \( \dot{V}(x) \) is not negative definite everywhere.
Only when \( x_{2} < 0 \), we can see that \( 2x_{1}^{2} x_{2} < 0 \) and thereby \( \dot{V}(x) < 0 \).
Thereby, the region of attraction is given by
\[
    \boxed{
        \mathcal{R} = \{ (x_1, x_2) \mid x_2 \leq 0 \}
    }
\]
To check for asymptotic stability, we can use LaSalle's invariance principle.
We first find the points where \( \dot{V}(x) = 0 \),
\[
    \implies
    -2(x_{1}^{2} + x_{2}^{2}) + 2x_{1}^{2} x_{2} = 0
    \implies
    x_{1}^{2} x_{2} = x_{1}^{2} + x_{2}^{2}
\]
Locally near the equilibrium point, we can see that the only solution to this equation is \( x_{1} = x_{2} = 0 \), thereby allowing us to conclude that the equilibrium point \underline{is asymptotically stable}, by LaSalle's invariance principle.
